cedar-lean/Cedar/TPE/Input.lean
@@ -62,11 +62,10 @@ def PartialEntities.attrs (es : PartialEntities) (uid : EntityUID) : Option (Map
 def partialIsValid {α} (o : Option α) (f : α → Bool) : Bool :=
   (o.map f).getD true
 
--- We do not check if `req`'s action is valid (i.e, if it's contained in `env`)
--- because this function is called after validation, which already ensures it
 def requestIsValid (env : Environment) (req : PartialRequest) : Bool :=
   (partialIsValid req.principal.asEntityUID λ principal =>
     instanceOfEntityType principal env.reqty.principal env.ets.entityTypeMembers?) &&
+  req.action == env.reqty.action &&
   (partialIsValid req.resource.asEntityUID λ resource =>
     instanceOfEntityType resource env.reqty.resource env.ets.entityTypeMembers?) &&
   (partialIsValid req.context λ m =>
